@prefix AT:    <http://data.ifpri.org/lod/at/resource/> .
@prefix crop:  <http://data.ifpri.org/lod/crop/> .

@prefix webprotege: <http://protege.stanford.edu/webprotege/> .
@prefix dc:    <http://purl.org/dc/elements/1.1/> .
@prefix dct:   <http://purl.org/dc/terms/> .
@prefix geo:   <http://aims.fao.org/aos/geopolitical.owl#> .
@prefix owl:   <http://www.w3.org/2002/07/owl#> .
@prefix rdf:   <http://www.w3.org/1999/02/22-rdf-syntax-ns#> .
@prefix rdfs:  <http://www.w3.org/2000/01/rdf-schema#> .
@prefix xsd:   <http://www.w3.org/2001/XMLSchema#> .

AT:     a                    owl:Ontology ;
        rdfs:comment         "Agricultural Technology ontology" , "This ontology was generated from an ontology revision in webprotege. See http://webprotege-beta.stanford.edu" ;
        webprotege:revision  264 ;
        dc:creator           "soonho" , "system" , "mbacou" , "guest" , "mcomanescu" ;
        dc:date              "Jul 28, 2013 6:56:15 AM"^^xsd:dateTime ;
        owl:imports          <http://aims.fao.org/aos/geopolitical.owl> , crop: .

#################### AT Classes

AT:Aflatoxins_related_postharvest_technology
        a                owl:Class ;
        rdfs:label       "Aflatoxins related postharvest technology"@en ;
        rdfs:subClassOf  AT:Food_safety_postharvest_technology .

AT:Agroforestry_technology
        a                owl:Class ;
        rdfs:label       "Agroforestry technology"@en ;
        rdfs:subClassOf  AT:Technology .

AT:Animal_biotechnology
        a                owl:Class ;
        rdfs:label       "Animal biotechnology"@en ;
        rdfs:subClassOf  AT:Germplasm_technology .

AT:Animal_health_and_disease_control
        a                owl:Class ;
        rdfs:label       "Animal health and disease control"@en ;
        rdfs:subClassOf  AT:Livestock_technology .

AT:Automated_disease_reporting
        a                owl:Class ;
        rdfs:label       "Automated disease reporting"@en ;
        rdfs:subClassOf  AT:Animal_health_and_disease_control .

AT:Bed_planting  a       owl:Class ;
        rdfs:subClassOf  AT:Crop_management_technology .

AT:Biofortification_technology
        a                owl:Class ;
        rdfs:subClassOf  AT:Plant_biotechnology .

AT:Biofortified_lentil_with_iron_and_zinc
        a                owl:Class ;
        rdfs:subClassOf  AT:Biofortification_technology .

AT:Biotechnology  a      owl:Class ;
        rdfs:label       "Biotechnology"@en ;
        rdfs:subClassOf  AT:Technology ;
        dc:description   "Biotechnology is the use of living systems and organisms to develop or make useful products, or \"any technological application that uses biological systems, living organisms or derivatives thereof, to make or modify products or processes for specific use (source: wikipedia)" .

AT:Blended_fertilizers
        a                owl:Class ;
        rdfs:comment     "Blended fertilizers are made by physically mixing fertilizer materials to give a desired grade. The individual particles remain separate in the mixture, and segregation may occur. This problem can be reduced by using materials with the same particle size. The quality of the blended fertilizer, particularly the segregation of the individual fertilizer materials, should be an important factor in choosing a fertilizer. Poor quality blends may contain the guaranteed nutrients but if there is segregation these nutrients will not be supplied uniformly to the crop. If properly made so as to reduce segregation during transportation and application, blends generally are equal in agronomic effectiveness to granulated complete fertilizers. Blends have the added advantage of allowing a very wide range of fertilizer grades, thus making it possible to match a fertilizer exactly to a soil test recommendation." ;
        rdfs:subClassOf  AT:Soil_management ;
        dc:source        "http://extension.psu.edu/agronomy-guide/cm/sec2/sec28d" .

AT:Breeding_method  a    owl:Class ;
        rdfs:subClassOf  AT:Method .

AT:Breeding_technology
        a                owl:Class ;
        rdfs:label       "Breeding technology"@en ;
        rdfs:subClassOf  AT:Livestock_technology .

AT:Climate_resilient_techology
        a                owl:Class ;
        rdfs:label       "Climate resilient cereals" ;
        rdfs:subClassOf  AT:Technology .

AT:Conservation_tillage
        a                owl:Class ;
        rdfs:comment     "Conservation tillage leaves at least 30% of crop residue on the soil surface, or at least 1,000 lb/ac (1,100 kg/ha) of small grain residue on the surface during the critical soil erosion period. This slows water movement, which reduces the amount of soil erosion. Conservation tillage also benefits farmers by reducing fuel consumption and soil compaction. By reducing the number of times the farmer travels over the field, farmers realize significant savings in fuel and labor. In most years since 1997, conservation tillage was used in US cropland more than intensive or reduced tillage" ;
        rdfs:subClassOf  AT:Crop_management_technology .

AT:Cost-effective_vaccine_production
        a                owl:Class ;
        rdfs:label       "Cost-effective vaccine production"@en ;
        rdfs:subClassOf  AT:Animal_health_and_disease_control .

AT:Crop_management_technology
        a                owl:Class ;
        rdfs:comment     "Technology related to the crop management defined as \"the art and science of controlling or directing crop production. Its objective is to provide useful food and fiber products for society at reasonable costs to the consumer and with an acceptable margin of profit for the producer.\"" ;
        rdfs:subClassOf  AT:Technology ;
        dc:source        "http://www.annualreviews.org/doi/abs/10.1146/annurev.py.20.090182.002223?journalCode=phyto" .

AT:Cropping  a           owl:Class ;
        rdfs:subClassOf  AT:Crop_management_technology .

AT:Direct-seeding  a     owl:Class ;
        rdfs:comment     "ransplanted rice has deleterious effects on the soil environment for the succeeding wheat and other upland crops. Direct seeded rice which removes puddling and drudgery of transplanting the young rice seedlings provides an option to resolve the adaphic conflict and enhance the sustainability of rice-wheat cropping system. Puddling requires lots of scarce water at a time when there is little water in the reservoirs, destroys soil structure and adversely affects soil productivity. DSR overcomes the problem of seasonality in labour requirement for rice nursery raising and transplanting operations.Non-development of ground water in kharif, late onset of monsoon and drudgery of operations often delays rice transplanting which leads to late vacation of fields, forcing farmers to plant wheat after the optimum sowing time. DSR facilitates timely establishment of rice and succeeding winter crops. Unlike puddle fields, DSR fields do not crack and thus help save irrigation water. Surface retained residue serve as physical barrier to emergence of weeds, moderate the soil temperature in summers and winters, conserve soil moisture, add organic matter and nutrients to the soil on decomposition." ;
        rdfs:subClassOf  AT:Water_management , AT:sowing_technology ;
        dc:source        "http://agropedia.iitk.ac.in/content/direct-seeded-rice" .

AT:Disease  a   owl:Class .

AT:Disease-resistant_bush_and_climbing_beans
        a                owl:Class ;
        rdfs:subClassOf  AT:Resistance_to_insect_pests_variety .

AT:Disease-resistant_early-maturing_cowpea_variety
        a                owl:Class ;
        rdfs:subClassOf  AT:Resistance_to_insect_pests_variety .

AT:Disease-resistant_early-maturing_peanut_variety
        a                owl:Class ;
        rdfs:subClassOf  AT:Resistance_to_insect_pests_variety .

AT:Early_maturing_rice_variety
        a                owl:Class ;
        rdfs:subClassOf  AT:High-yielding_cereal_variety .

AT:Early_wheat_sowing
        a                owl:Class ;
        rdfs:subClassOf  AT:sowing_technology .

AT:Economic_and_policy_technology
        a                owl:Class ;
        rdfs:label       "Economic and policy technology"@en ;
        rdfs:subClassOf  AT:Technology .

AT:Educational_technology
        a                owl:Class ;
        rdfs:label       "Educational technology"@en ;
        rdfs:subClassOf  AT:Technology .

AT:Energy_technology  a  owl:Class ;
        rdfs:label       "Energy technology"@en ;
        rdfs:subClassOf  AT:Technology .

AT:Extra_early_lentil_variety
        a                owl:Class ;
        rdfs:subClassOf  AT:Highly_productive_grain_legume_variety .

AT:Fallow_management  a  owl:Class ;
        rdfs:subClassOf  AT:Crop_management_technology .

AT:Fertilizer_Deep_Placement
        a                owl:Class ;
        rdfs:comment     "FDP as a more effective alternative to the traditional method of applying fertilizer by surface broadcasting (spreading, usually by hand) across a field or paddy. FDP is an innovative, proven fertilizer application technology that achieves average yield increases of 18 percent while reducing fertilizer use by about one-third. (FDP is known as urea deep placement, or UDP, when only urea is applied.) FDP consists of two key components. The first is a fertilizer ‘briquette,’ produced by compacting commercially available solid fertilizers." ;
        rdfs:subClassOf  AT:Soil_management ;
        dc:source        "http://www.ifdc.org/Technologies/Fertilizer-Deep-Placement-(FDP)/" .

AT:Fertilizer_technology
        a                owl:Class ;
        rdfs:label       "Fertilizer technology"@en ;
        rdfs:subClassOf  AT:Technology ;
        dc:source        <http://aims.fao.org/aos/agrovoc/c_27895> .

AT:Fighting_invasive_species_in_drylands
        a                owl:Class ;
        rdfs:label       "Fighting invasive species in drylands" ;
        rdfs:subClassOf  AT:Rangeland_management .

AT:Fishery_technology
        a                owl:Class ;
        rdfs:label       "Fishery technology"@en ;
        rdfs:subClassOf  AT:Technology .

AT:Food_Preservation  a  owl:Class ;
        rdfs:label       "Food Preservation"@en ;
        rdfs:subClassOf  AT:Food_technology .

AT:Food_Processing  a    owl:Class ;
        rdfs:label       "Food Processing"@en ;
        rdfs:subClassOf  AT:Food_technology .

AT:Food_safety_postharvest_technology
        a                owl:Class ;
        rdfs:label       "Food safety postharvest technology"@en ;
        rdfs:subClassOf  AT:Postharvest_technology ;
        dc:description   "water contamination from waste-water for vegetables and fruits\n\nsource:f" , "water contamination from waste-water for vegetables and fruits" ;
        dc:source        <https://asset1.basecamp.com/1766833/projects/528208-caadp-cgiar-mapping/attachments/34150405/44900a604d8b84945ada1d2b996031b09be8abe7/original/Response%20from%20CGIAR%20to%20USAID%20Request%20for%20comments%20on%20Scalable%20Agricultural%20Technologies%20-01-07-2013.pd> .

AT:Food_technology  a    owl:Class ;
        rdfs:label       "Food technology"@en ;
        rdfs:subClassOf  AT:Technology .

AT:Forage_Seed_Multiplication_Sites
        a                owl:Class ;
        rdfs:label       "Forage Seed Multiplication Sites" ;
        rdfs:subClassOf  AT:Forage_and_feed_technology .

AT:Forage_and_feed_distribution_networks
        a                owl:Class ;
        rdfs:label       "Forage and feed distribution networks" ;
        rdfs:subClassOf  AT:Forage_and_feed_technology .

AT:Forage_and_feed_technology
        a                owl:Class ;
        rdfs:label       "Forage and feed technology" ;
        rdfs:subClassOf  AT:Livestock_technology .

AT:Gene_preservation_of_local_dryland_livestock
        a                owl:Class ;
        rdfs:label       "Gene preservation of local dryland livestock" ;
        rdfs:subClassOf  AT:Breeding_technology .

AT:Germplasm_technology
        a                owl:Class ;
        rdfs:subClassOf  AT:Biotechnology ;
        dc:description   "Any technology related to germplams which is defined as a collection of genetic resources for an organism" .

AT:High-iron_bean  a     owl:Class ;
        rdfs:subClassOf  AT:Biofortification_technology .

AT:High-iron_pearl_millet
        a                owl:Class ;
        rdfs:subClassOf  AT:Biofortification_technology .

AT:High-yielding_cereal_variety
        a                owl:Class ;
        rdfs:subClassOf  AT:Quality_and_yield_improving .

AT:High-yielding_chickpea_varietiy
        a                owl:Class ;
        rdfs:label       "High-yielding chickpea varieties"@en ;
        rdfs:subClassOf  AT:Highly_productive_grain_legume_variety ;
        dc:description   "25% yield gains for almost 4.5 million farm families each farming an average of roughly 1 ha; New varieties would yield $370-$540/ha in East Africa and $375-$450/ha in South \nAsia (India, Bangladesh, Burma)" .

AT:High-yielding_chickpea_variety
        a                owl:Class ;
        rdfs:subClassOf  AT:Highly_productive_grain_legume_variety .

AT:High-yielding_climbing_bean_variety
        a                owl:Class ;
        rdfs:subClassOf  AT:Highly_productive_grain_legume_variety .

AT:High-yielding_groundnut_variety
        a                owl:Class ;
        rdfs:subClassOf  AT:High-yielding_nut_variety .

AT:High-yielding_nut_variety
        a                owl:Class ;
        rdfs:subClassOf  AT:Quality_and_yield_improving .

AT:High-yielding_pigeon_pea_variety
        a                owl:Class ;
        rdfs:label       "High-yielding pigeon pea varieties"@en ;
        rdfs:subClassOf  AT:Highly_productive_grain_legume_variety ;
        dc:description   "Large seeded, high yielding pigeon pea. Yields from 1.5 to 3.5 tons/ha. New varieties would yield $185-325/ha in East and Southern Africa, and $130-$255/ha in India and Myanmar."@en .

AT:High_yield_Kharif_maize_variety
        a                owl:Class ;
        rdfs:subClassOf  AT:High-yielding_cereal_variety .

AT:Highly_productive_grain_legume_variety
        a                owl:Class ;
        rdfs:comment     "<p style=\"margin-top: 0\">\n      The grain legume is customized classification based on their usage.\n    </p>\n    <p style=\"margin-top: 0\">\n      More information--&gt; \n      http://www.hort.purdue.edu/newcrop/proceedings1990/v1-154.html#Table 3\n    </p>" ;
        rdfs:subClassOf  AT:Highly_productive_legume_variety .

AT:Highly_productive_legume_variety
        a                owl:Class ;
        rdfs:label       "Highly productive grain legumes" ;
        rdfs:subClassOf  AT:Quality_and_yield_improving .

AT:Holistic_resource_management
        a                owl:Class ;
        rdfs:label       "Holistic resource management (HRM)" ;
        rdfs:subClassOf  AT:Rangeland_management ;
        dc:description   "Holistic management iin agriculture is a systems thinking approach to managing resources that was originally developed by Allan Savory for reversing desertification."@en ;
        dc:source        "Allan Savory, Jody Butterfield (1998) Holistic Management: A New Framework for Decision Making, Island Press, 1998"@en .

AT:Hybrid_guinea-type_sorghum_variety
        a                owl:Class ;
        rdfs:subClassOf  AT:High-yielding_cereal_variety .

AT:Hybrid_maize_variety
        a                owl:Class ;
        rdfs:label       "Hybrid maize varieties"@en ;
        rdfs:subClassOf  AT:High-yielding_cereal_variety .

AT:Hybrid_pearl_millet_variety
        a                owl:Class ;
        rdfs:subClassOf  AT:High-yielding_cereal_variety .

AT:Hybrid_white_and_yellow_maize_variety
        a                owl:Class ;
        rdfs:subClassOf  AT:High-yielding_cereal_variety .

AT:Identification_of_camel_diseases
        a                owl:Class ;
        rdfs:label       "Identification of camel diseases" ;
        rdfs:subClassOf  AT:Automated_disease_reporting .

AT:Information_and_communication_technology
        a                owl:Class ;
        rdfs:label       "Information and communication technology"@en ;
        rdfs:subClassOf  AT:Technology .

AT:Integrated_soil_fertility_management
        a                owl:Class ;
        rdfs:label       "Integrated soil fertility management (ISFM)" ;
        rdfs:subClassOf  AT:Information_and_communication_technology .

AT:Integrated_weed_management
        a                owl:Class ;
        rdfs:subClassOf  AT:Crop_management_technology .

AT:Intercropping  a      owl:Class ;
        rdfs:subClassOf  AT:Cropping .

AT:Intercropping_banana_and_coffee_system
        a                owl:Class ;
        rdfs:subClassOf  AT:System .

AT:Intergovernmental_organizations
        a                owl:Class ;
        rdfs:subClassOf  AT:International_organization ;
        dc:description   "the type of organization most closely associated with the term 'international organization', these are organizations that are made up primarily of sovereign states (referred to as member states). Notable examples include the United Nations (UN), Organisation for Economic Co-operation and Development (OECD) Organization for Security and Co-operation in Europe (OSCE), Council of Europe (CoE), European Union (EU; which is a prime example of a supranational organization), and World Trade Organization (WTO)." .

AT:International_organization
        a                owl:Class ;
        rdfs:subClassOf  AT:Organization .

AT:Livestock_identification_and_traceability
        a                owl:Class ;
        rdfs:label       "Livestock identification and traceability" ;
        rdfs:subClassOf  AT:Livestock_technology .

AT:Livestock_insurance
        a                owl:Class ;
        rdfs:label       "Livestock insurance" ;
        rdfs:subClassOf  AT:Livestock_technology .

AT:Livestock_technology
        a                owl:Class ;
        rdfs:label       "Livestock technology"@en ;
        rdfs:subClassOf  AT:Technology .

AT:Local_participation_in_breed_enhancement
        a                owl:Class ;
        rdfs:label       "Local participation in breed enhancement" ;
        rdfs:subClassOf  AT:Breeding_technology .

AT:Long_duration_and_high-yielding_wheat_variety
        a                owl:Class ;
        rdfs:subClassOf  AT:High-yielding_cereal_variety .

AT:Low_ODAP_grass_pea_variety
        a                owl:Class ;
        rdfs:comment     "<p style=\"margin-top: 0\">\n      There is no defined classification about grass pea is a kind of grain \n      legume. So, for now, we put this class under general legume class.\n    </p>" ;
        rdfs:subClassOf  AT:Highly_productive_grain_legume_variety .

AT:Machine_transplanting
        a                owl:Class ;
        rdfs:subClassOf  AT:Crop_management_technology .

AT:Method  a    owl:Class .

AT:Mixed_cropping  a     owl:Class ;
        rdfs:comment     "growing of two or more crops simultaneously on the same piece of land" ;
        rdfs:subClassOf  AT:Cropping .

AT:Mixed_cropping_climate_resilient_system
        a                owl:Class ;
        rdfs:subClassOf  AT:System .

AT:Mobile_Market_Information_Systems
        a                owl:Class ;
        rdfs:label       "Mobile Market Information Systems"@en ;
        rdfs:subClassOf  AT:Mobile_technology .

AT:Mobile_technology  a  owl:Class ;
        rdfs:label       "Mobile technology"@en ;
        rdfs:subClassOf  AT:Information_and_communication_technology .

AT:Nanotechnology  a     owl:Class ;
        rdfs:label       "Nanotechnology"@en ;
        rdfs:subClassOf  AT:Technology ;
        dc:description   "the manipulation of matter on an atomic and molecular scale" .

AT:Nitrogen-use_efficient_rice-hybrid
        a                owl:Class ;
        rdfs:subClassOf  AT:High-yielding_cereal_variety .

AT:No-till  a            owl:Class ;
        rdfs:comment     "Never use a plow, disk, etc. ever again. Aims for 100% ground cover." ;
        rdfs:subClassOf  AT:Conservation_tillage .

AT:Nutritional_quality
        a                owl:Class ;
        rdfs:label       "Nutritional quality"@en ;
        rdfs:subClassOf  AT:Postharvest_technology ;
        dc:description   "some work on orange-fleshed sweet potatoes by CIP and putting together cereals with pulses – cassava with soybean and cowpea by IITA and probably other examples)\n\nsource:f" .

AT:Optimized_breed_selection_of_local_dryland_livestock
        a                owl:Class ;
        rdfs:label       "" ;
        rdfs:subClassOf  AT:Breeding_technology .

AT:Orange_fleshed_sweet_potato
        a                owl:Class ;
        rdfs:subClassOf  AT:Biofortification_technology .

AT:Organization  a  owl:Class .

AT:Orobanche_tolerant_fava_bean_variety
        a                owl:Class ;
        rdfs:subClassOf  AT:Resistance_to_fungi_variety .

AT:Pathogen  a          owl:Class ;
        dc:description  "a microorganism—in the widest sense, such as a virus, bacterium, prion, or fungus—that causes disease in its host. The host may be an animal (including humans), a plant, or even another microorganism" .

AT:Payments_for_eco-systems_services
        a                owl:Class ;
        rdfs:label       "Payments for eco-systems services" ;
        rdfs:subClassOf  AT:Rangeland_management .

AT:Perishable_products_for_food_safety
        a                owl:Class ;
        rdfs:label       "Perishable products for food safety"@en ;
        rdfs:subClassOf  AT:Food_safety_postharvest_technology ;
        dc:creator       "John McDermott" ;
        dc:description   "packages of food safety improvements for milk in South Asia and East Africa linked to capacity building of informal market agents by NGOs (Delia Grace and colleagues at ILRI could provide numbers on potential scale in South Asia and East Africa and on efforts currently under way)" ;
        dc:source        <https://asset1.basecamp.com/1766833/projects/528208-caadp-cgiar-mapping/attachments/34150405/44900a604d8b84945ada1d2b996031b09be8abe7/original/Response%20from%20CGIAR%20to%20USAID%20Request%20for%20comments%20on%20Scalable%20Agricultural%20Technologies%20-01-07-2013.pdf> .

AT:Plant_biotechnology
        a                owl:Class ;
        rdfs:label       "Plant biotechnology"@en ;
        rdfs:subClassOf  AT:Germplasm_technology .

AT:Postharvest_technology
        a                owl:Class ;
        rdfs:label       "Postharvest technology"@en ;
        rdfs:subClassOf  AT:Technology ;
        dc:description   "In agriculture, postharvest handling is the stage of crop production immediately following harvest, including cooling, cleaning, sorting and packing. The instant a crop is removed from the ground, or separated from its parent plant, it begins to deteriorate. Postharvest treatment largely determines final quality, whether a crop is sold for fresh consumption, or used as an ingredient in a processed food product." ;
        dc:source        "Wikipedia http://en.wikipedia.org/wiki/Postharvest" ;
        owl:versionInfo  "TODO: " .

AT:Pre-breeding_method
        a                owl:Class ;
        rdfs:subClassOf  AT:Method .

AT:Private_sector_animal_health_delivery_systems
        a                owl:Class ;
        rdfs:label       "Private sector animal health delivery systems"@en ;
        rdfs:subClassOf  AT:Animal_health_and_disease_control .

AT:Protection_technology
        a                owl:Class ;
        rdfs:label       "Protection technology"@en ;
        rdfs:subClassOf  AT:Technology .

AT:Provitamin_A_cassava
        a                owl:Class ;
        rdfs:subClassOf  AT:Biofortification_technology .

AT:Provitamin_A_maize
        a                owl:Class ;
        rdfs:subClassOf  AT:Biofortification_technology .

AT:Purdue_Improved_Crop_Storage_bag
        a                owl:Class ;
        rdfs:comment     "PICS bag rovides a simple, low-cost method of reducing post-harvest cowpea (Vigna unguiculata) losses due to bruchid infestations in west and central Africa.\nA PICS bag consists of two layers of polyethylene bags, these are then surrounded by a third layer of woven polypropylene,[3] thereby creating a hermetically sealed environment in which harvested cowpeas are stored. This oxygen-deprived environment proves fatal for Bruchidius atrolineatus[4] and Calloso bruchus maculatus." ;
        rdfs:subClassOf  AT:Postharvest_technology ;
        dc:source        "http://en.wikipedia.org/wiki/Purdue_Improved_Crop_Storage_(PICS)_bags" .

AT:Quality_and_yield_improving
        a                owl:Class ;
        rdfs:subClassOf  AT:Plant_biotechnology .

AT:Rangeland_management
        a                owl:Class ;
        rdfs:label       "Rangeland management" ;
        rdfs:subClassOf  AT:Livestock_technology .

AT:Resistance_to_bacteria_GMO
        a                owl:Class ;
        rdfs:subClassOf  AT:Resistance_to_bacteria_variety .

AT:Resistance_to_bacteria_variety
        a                owl:Class ;
        rdfs:subClassOf  AT:Resistance_to_pests_and_diseases .

AT:Resistance_to_fungi_variety
        a                owl:Class ;
        rdfs:subClassOf  AT:Resistance_to_pests_and_diseases .

AT:Resistance_to_insect_pests_variety
        a                owl:Class ;
        rdfs:subClassOf  AT:Resistance_to_pests_and_diseases .

AT:Resistance_to_pests_and_diseases
        a                owl:Class ;
        rdfs:subClassOf  AT:Plant_biotechnology .

AT:Resistance_to_virus_variety
        a                owl:Class ;
        rdfs:subClassOf  AT:Resistance_to_pests_and_diseases .

AT:Rust_resistant_wheat_variety
        a                owl:Class ;
        rdfs:subClassOf  AT:Resistance_to_virus_variety .

AT:Safe-use_of_pesticides
        a                owl:Class ;
        rdfs:label       "Safe-use of pesticides" ;
        rdfs:subClassOf  AT:Food_safety_postharvest_technology ;
        dc:description   "some initial work by IRRI and CIP several years ago). Private sector working with small scale producers in different contexts. Somebody would need to check with the private sector if of interest" ;
        dc:source        <https://asset1.basecamp.com/1766833/projects/528208-caadp-cgiar-mapping/attachments/34150405/44900a604d8b84945ada1d2b996031b09be8abe7/original/Response%20from%20CGIAR%20to%20USAID%20Request%20for%20comments%20on%20Scalable%20Agricultural%20Technologies%20-01-07-2013.pdf> .

AT:Soil_management  a    owl:Class ;
        rdfs:subClassOf  AT:Crop_management_technology .

AT:Strip-Till  a         owl:Class ;
        rdfs:comment     "Narrow strips are tilled where seeds will be planted, leaving the soil in between the rows untilled." ;
        rdfs:subClassOf  AT:Conservation_tillage .

AT:System  a    owl:Class .

AT:Technology  a        owl:Class ;
        rdfs:comment    "the application of the knowledge and usage of tools (such as machines or utensils) and techniques to control one's environment)"@en ;
        rdfs:label      "Technology" ;
        dc:description  "the application of the knowledge and usage of tools and techniques to resolve practical problems"@en ;
        dc:source       <http://aims.fao.org/aos/agrovoc/c_7644> .

AT:Tolerance_to_herbicides
        a                owl:Class ;
        rdfs:subClassOf  AT:Plant_biotechnology .

AT:Transgenic_bananas_resistant_to_Xanthomonas_wilt_disease
        a                owl:Class ;
        rdfs:subClassOf  AT:Resistance_to_bacteria_variety .

AT:Triple_cropping  a    owl:Class ;
        rdfs:subClassOf  AT:Mixed_cropping .

AT:Vertisol_drainage_solution
        a                owl:Class ;
        rdfs:subClassOf  AT:Soil_management .

AT:Virus_resistant_locally_adapted_cassava
        a                owl:Class ;
        rdfs:label       "Virus resistant locally adapted cassava"@en ;
        rdfs:subClassOf  AT:Resistance_to_virus_variety ;
        dc:description   "Combined CMD and CBSD varieties." .

AT:Waste-water_treatment
        a                owl:Class ;
        rdfs:label       "Waste-water treatment" ;
        rdfs:subClassOf  AT:Water_management_technology ;
        dc:description   "water contamination from waste-water for vegetables and fruits (IWMI is working on business plans for better management of grey water – Pay Drechsel is leading this and could be linked to value chain work)" .

AT:Water_management  a   owl:Class ;
        rdfs:subClassOf  AT:Crop_management_technology .

AT:Water_management_technology
        a                owl:Class ;
        rdfs:subClassOf  AT:Technology .

AT:Wood_technology  a    owl:Class ;
        rdfs:label       "Wood technology"@en ;
        rdfs:subClassOf  AT:Technology .
AT:organization  a  owl:Class .

AT:rhizobial_inoculant
        a                owl:Class ;
        rdfs:comment     "Inoculating legumes with rhizobia can achieve substantial increases in legume nodulation, grain and \nbiomass yield, nitrogen fixation and post-crop soil nitrate levels" ;
        rdfs:subClassOf  AT:Soil_management ;
        dc:source        "http://www.grdc.com.au/~/media/B943F697AF9A406ABBA20E136FDB7DC4.pdf" .

AT:sowing_technology  a  owl:Class ;
        rdfs:comment     "technology related to the process of planting seeds" ;
        rdfs:subClassOf  AT:Crop_management_technology .

#################### AT properties

AT:hasCoverage  a    owl:ObjectProperty ;
        rdfs:domain  AT:Technology ;
        rdfs:range   geo:area .

AT:hasTargetCrop  a    owl:ObjectProperty ;
        rdfs:domain    AT:Plant_biotechnology ;
        rdfs:range     crop:Crop ;
        owl:inverseOf  AT:isTargetCropOf .

AT:international_nongovernmental_organization
        a                owl:Class ;
        rdfs:subClassOf  AT:International_organization ;
        dc:description   "non-governmental organizations (NGOs) that operate internationally" .

AT:isTargetCropOf  a   owl:ObjectProperty ;
        rdfs:domain    crop:Crop ;
        rdfs:range     AT:Plant_biotechnology ;
        owl:inverseOf  AT:hasTargetCrop .

AT:is_developed_by  a  owl:ObjectProperty ;
        rdfs:domain  AT:Technology ;
        rdfs:range   AT:Organization .

#################### AT individuals

AT:name_  a               AT:Hybrid_guinea-type_sorghum_variety ;
        AT:hasTargetCrop  crop:Sorghum .

AT:Hybrid_maize_variety_7
        a                 AT:Hybrid_maize_variety ;
        AT:hasTargetCrop  crop:Maize .

#################### External terms

crop:   rdfs:label       "Agricultural Ontology Version 1" ;
        dc:creator       "HarvestChoice" ;
        dc:description   "Agricultural ontology for CRP mapping" ;
        dct:modified     "2014-05-11" ;
        owl:versionInfo  "1.0" .

crop:Crop  a    rdfs:Class .

crop:Maize  AT:isTargetCropOf  AT:Hybrid_maize_variety_7 .

crop:Sorghum  AT:isTargetCropOf  AT:name_ .

dc:creator  a   owl:AnnotationProperty .

dc:description  a  owl:AnnotationProperty .

dc:identifier  a  owl:AnnotationProperty .

dc:source  a    owl:AnnotationProperty .
