# prefix for for a "spatio-temporal Datacube" extension to qb
@prefix qb4st: <http://www.w3.org/ns/qb4st/> .

# a canonical spatial concept ontology (update to SDW output )
# we cannot have this as a dependency until accepted as a Note or Rec - so we declare equivalence 
# @prefix so: <http://geosemweb.net/sdwgeo#> .

# a canonical time concept ontology (update to SDW output )
@prefix time: <http://www.w3.org/2006/time#> .


@prefix : <http://resources.opengeospatial.org/def/qbcomponents/qb4st> .

@prefix rdf:            <http://www.w3.org/1999/02/22-rdf-syntax-ns#> .
@prefix rdfs:           <http://www.w3.org/2000/01/rdf-schema#> .
@prefix owl:            <http://www.w3.org/2002/07/owl#> .
@prefix xsd:            <http://www.w3.org/2001/XMLSchema#> .
@prefix skos:           <http://www.w3.org/2004/02/skos/core#> .
@prefix qb:             <http://purl.org/linked-data/cube#> .
@prefix dct:        	<http://purl.org/dc/terms/> .
@prefix foaf: 			<http://xmlns.com/foaf/0.1/>.
#########################

#
# Ontology definitions - mainly to provide Linked Data resources 
#
#########################

<http://resources.opengeospatial.org/def/qbcomponents/qb4st> a owl:Ontology;
   dct:creator [ foaf:mbox  <mailto:rob@metalinkage.com.au>; foaf:name "Rob Atkinson"; ];

	dct:created "2016-10-25"^^xsd:date ;
	dct:license <https://creativecommons.org/licenses/by/4.0/> ;
	rdfs:label "QB4ST: Spatial Temporal Datacube Extensions"@en;
	dct:rights "Copyright Â© 2016 W3C All Rights Reserved. W3C liability, trademark and document use rules apply."@en ;
	rdfs:comment "QB4ST defines a minimal set of definitions for spatio-temporal properties of RDF Datacube elements and base abstract classes to allow disocvery of spatio-temporal aspects of a dataset described using RDF datacube"@en;
	# owl:imports 
	owl:versionIRI <http://www.w3.org/2006/time#2016> 
.

#########################
#
# Abstract concept definitions - provides a hook for alignment with future standards for defining general spatial concepts 
#
#########################



qb4st:SpatialThing a rdfs:Class, owl:Class ;
	rdfs:label "Spatial Thing"@en ;
	rdfs:comment "This is defined here pending availability of a canonical definition of spatial concepts - at which point an equivalence will be declared"@en ;
.

qb4st:Point  a rdfs:Class, owl:Class ;
	rdfs:label "Geometric Point"@en ;
	rdfs:comment "This is defined here pending availability of a canonical definition of spatial concepts - at which point an equivalence will be declared"@en ;
.


qb4st:CRS a rdfs:Class, owl:Class ;
	rdfs:label "Coordinate Reference System"@en ;
	rdfs:comment "This is defined here pending availability of a canonical definition of spatial concepts - at which point an equivalence will be declared"@en ;
.


qb4st:AnyNumber a rdfs:Class, owl:Class ;
      rdfs:label "Any number"@en ;      
      rdfs:comment "A datatype that is the union of numeric xsd data types. equivalent to the xsd specification that uses an xsd:union of memberTypes='xsd:decimal xsd:double xsd:float xsd:integer'."@en ;
      owl:equivalentClass [ 
		rdf:type  rdfs:Datatype;
		owl:unionOf (xsd:float xsd:decimal xsd:integer xsd:double) 
      ]
.

##################
#
# qb:ComponentProperty specialisations 
#
# These extend the RDF-QB model through the presence of one or more spatio-temporal attributes bound to the specific component 
# (as opposed to qb:AttributeMeasure properties which belong to the whole DataSet, Slice or Observation (subclasses of qb:Attachable)
#
##################

qb4st:SpatialProperty a rdfs:Class, owl:Class;
	rdfs:subClassOf rdfs:Property, qb:ComponentProperty ;
	rdfs:label "Abstract Spatial Property"@en ;
	rdfs:comment "A generalised spatial property - defines how properties like CRS, accuracy and precision can be applied to any spatial value in a dimension of measure"@en ;
	rdfs:subClassOf [
        a owl:Restriction ;
        owl:onProperty qb:concept ;
        owl:someValuesFrom qb4st:SpatialThing ;
     ]  ;
	 . 

qb4st:TemporalProperty a rdfs:Class, owl:Class;
	rdfs:subClassOf rdfs:Property, qb:ComponentProperty ;
	rdfs:label "Abstract Spatial Property"@en ;
	rdfs:comment "A generalised temporal property, requires rdfs:range of the property to be a time:Interval"@en ;
	rdfs:subClassOf [
        a owl:Restriction ;
        owl:onProperty rdfs:range ;
        owl:someValuesFrom time:Interval ;
     ]  ;
	 . 
	 
qb4st:SpatialDimension a rdfs:Class, owl:Class; 
	rdfs:label "Spatial Dimension"@en ;
	rdfs:subClassOf qb:DimensionProperty, qb4st:SpatialProperty;
	rdfs:comment "A generalised spatial dimension - defines common usage of a concept for a spatial dimension, and hence potential transformability between instances."@en
	. 
	

qb4st:CoordDimension a rdfs:Class, owl:Class;
	rdfs:subClassOf qb4st:SpatialDimension;
	rdfs:label "Abstract Numerical Coordinate Dimension"@en ;
	rdfs:comment "A numeric coordinate dimension. NB - this is a dimension - an index with spatial semantics whose value represents . If an actual location is being measured, use a coordMeasure"@en;
	rdfs:subClassOf [
        a owl:Restriction ;
        owl:onProperty rdfs:range  ;
        owl:someValuesFrom qb4st:AnyNumber  ;
     ]  ;
	 . 	 


qb4st:RefArea a  rdfs:Class, owl:Class ;
	rdfs:subClassOf qb4st:SpatialDimension, qb:CodedProperty ;
	rdfs:label "Location by spatial Feature"@en ;
	rdfs:comment "Spatial context identified by a Spatial Feature. As a dimension, it is used as an index, and may not be missing or multi-valued. Such a property is both a spatial property and a CodedProperty. Note this must also have a codelist defined, and thus each Feature is regarded as a skos:Concept"@en ;
	rdfs:subClassOf [
        a owl:Restriction ;
        owl:onProperty rdfs:range  ;
        owl:someValuesFrom qb4st:Feature  ;
     ]  ;
	.

qb4st:SpatialMeasure a  rdfs:Class, owl:Class;
	rdfs:subClassOf qb:MeasureProperty;
	rdfs:label "abstract measure of spatial location"@en
	.

qb4st:PositionMeasure a  rdfs:Class, owl:Class ;
	rdfs:subPropertyOf qb4st:SpatialMeasure ;
	rdfs:label "Location by Point Coordinates"@en ;
	rdfs:comment "a measure of location as a Point (i.e. a complex spatial data type)"@en ;
		rdfs:subClassOf [
        a owl:Restriction ;
        owl:onProperty rdfs:range  ;
        owl:someValuesFrom qb4st:Point  ;
     ]  ;
	.

qb4st:CoordMeasure a  rdfs:Class, owl:Class ;
	rdfs:subPropertyOf qb4st:SpatialMeasure ;
	rdfs:label "Location partially recorded by a single Coordinate"@en ;
	rdfs:comment "Abstract class for partial measure of location as a single Coordinate - such as latitude"@en;
	rdfs:subClassOf [
        a owl:Restriction ;
        owl:onProperty rdfs:range  ;
        owl:someValuesFrom qb4st:AnyNumber  ;
     ]  ;
	.

qb4st:RefAreaMeasure a  rdfs:Class, owl:Class ;
	rdfs:subPropertyOf qb4st:SpatialMeasure, qb:CodedProperty ;
	rdfs:label "Location by spatial Feature"@en ;
	rdfs:comment "a measure of location as being with the bounds of an identified Spatial Feature. As a measure, it is not used as an index, and may be missing or multi-valued. Such a property is both a spatial property and a CodedProperty"@en ;
		rdfs:subClassOf [
        a owl:Restriction ;
        owl:onProperty rdfs:range  ;
        owl:someValuesFrom qb4st:Feature  ;
     ]  ;
	.

########################
#
# attributes of spatio-temporal components
#
# note the domain and range are not narrowly defined in general, allowing these properties to be re-used anywhere. For the same reason these are not defined
# as sub-properties of qb:ComponentProperty (specifically qb:AttributeProperty) in order to avoid inappropriate RDFS inferences
#
####################### 


qb4st:srs a rdfs:Property, owl:ObjectProperty;
	# meta:domainIncludes qb4st:SpatialProperty, qb4st:SpatialComponentSpecification;
	rdfs:label "Spatial Reference System"@en;
	rdfs:comment "Generalised Spatial Reference System - specific types may be coordinate, grid or feature based "@en
	.
	
qb4st:crs a rdfs:Property, owl:ObjectProperty;
	# meta:domainIncludes qb4st:SpatialProperty, qb4st:SpatialComponentSpecification;
	rdfs:subPropertyOf qb4st:srs ;	
	rdfs:range qb4st:CRS ;
	rdfs:label "CRS binding for a component specification or a property"@en;
	rdfs:comment "Allows declaration of a CRS for any spatial propert -- do we want to leave domain open? Leaves it to a general spatial ontology to handle if CRS is a canonical URI set , or dereferences to anything specific)"@en
	.

qb4st:crsaxis a rdfs:Property;
	# meta:domainIncludes qb4st:SpatialProperty, qb4st:SpatialComponentSpecification;
	rdfs:label "CRS axis element name"@en;
	rdfs:comment "Names a specific axis of the CRS, using the internal name of the CRS specified by the qb4st:crs property. Note that the data model for describing CRS is not defined at this point."@en
	.

qb4st:crslabel a rdfs:Property;
	# meta:domainIncludes qb4st:SpatialProperty, qb4st:SpatialComponentSpecification;
	rdfs:label "CRS label"@en;
	rdfs:comment "Provides a human readable name for the CRS - required because the dereferencing of a CRS identifier to access this information is not defined."@en
	.

qb4st:resolution a rdfs:Property;
	# meta:domainIncludes qb4st:CoordDimension , qb4st:SpatialComponentSpecification ;
	rdfs:range qb4st:AnyNumber ;
	rdfs:label "Resolution (Granularity)" ;
	rdfs:comment "Dimensions are indexes, a coordDimension specifies the granular partitioning of the coordinate space represented."@en
	.

qb4st:subdivides a rdfs:Property;
	# meta:domainIncludes qb4st:CoordDimension , qb4st:SpatialComponentSpecification ;
	rdfs:range qb4st:SpatialDimension ;
	rdfs:domain qb4st:SpatialDimension ;
	rdfs:label "Sub-divides" ;
	rdfs:comment "Indicates that the subject  dimension property is bound to feature identifiers that are sub-divisions of the features used by the object dimension property. This menas applications do not need to download either information models or feature sets to determine this critical relationship, nor rely on complex spatial operations."@en
	.	


#########################
#
# Data Structure - defines classes to allow inferencing and/or assertion that a dataset is in fact a spatio-temporal dataset 
#
#########################

qb4st:SpatialDSD a rdfs:Class, owl:Class;
	rdfs:subClassOf qb:DataStructureDefinition ;
	rdfs:label "Spatial Data Structure Definition"@en ;
	rdfs:comment "Specifies a data set includes one or more spatial properties, either in its organising dimension or its observed values"@en ;
	rdfs:subClassOf [
        a owl:Restriction ;
        owl:onProperty qb:component ;
        owl:someValuesFrom qb4st:SpatialComponentSpecification ;
     ]  ;
.

qb4st:TemporalDSD a rdfs:Class, owl:Class;
	rdfs:subClassOf qb:DataStructureDefinition ;
	rdfs:label "Spatial Data Structure Definition"@en ;
	rdfs:comment "Specifies a data set includes one or more temporal properties, either in its organising dimension or its observed values"@en ;
	rdfs:subClassOf [
        a owl:Restriction ;
        owl:onProperty qb:component ;
        owl:someValuesFrom qb4st:TemporalComponentSpecification ;
     ]  ;
.

qb4st:SpatioTemporalDSD a rdfs:Class, owl:Class;
	rdfs:subClassOf qb4st:SpatialDSD , qb4st:TemporalDSD;
	rdfs:label "Spatial-Temporal Data Structure Definition"@en ;
	rdfs:comment "Specifies a data set includes both spatial and temporal properties, either in its organising dimensions or its observed values"@en ;

.

qb4st:SpatialComponentSpecification a rdfs:Class, owl:Class;
	rdfs:subClassOf qb:ComponentSpecification ;
	rdfs:label "Spatial Component"@en ;
	rdfs:comment "A generalised spatial property - allows properties like CRS, bounds, accuracy and precision to be define for a spatial dimension or measure"@en ;
	rdfs:subClassOf [
        a owl:Restriction ;
        owl:onProperty qb:componentProperty;
        owl:someValuesFrom qb4st:SpatialProperty ;
     ]  ;
.

qb4st:TemporalComponentSpecification a rdfs:Class, owl:Class;
	rdfs:subClassOf qb:ComponentSpecification ;
	rdfs:label "Spatial Component"@en ;
	rdfs:comment "A generalised spatial property - allows properties like CRS, bounds, accuracy and precision to be define for a spatial dimension or measure"@en ;
	rdfs:subClassOf [
        a owl:Restriction ;
        owl:onProperty qb:componentProperty;
        owl:someValuesFrom qb4st:TemporalProperty ;
     ]  ;
.

# many not need these - unless we want to ask if a dataset has a spatial dimension vs a measure?
qb4st:SpatialDimensionComponentSpecification a rdfs:Class, owl:Class;
	rdfs:subClassOf qb:ComponentSpecification ;
	rdfs:label "Spatial Dimension Component"@en ;
	rdfs:comment "Allows identification of datasets organised using discrete spatial dimensions"@en ;
	rdfs:subClassOf [
        a owl:Restriction ;
        owl:onProperty qb:dimension;
        owl:someValuesFrom qb4st:SpatialDimension ;
     ]  ;
.

qb4st:SpatialMeasureComponentSpecification a rdfs:Class, owl:Class;
	rdfs:subClassOf qb:ComponentSpecification ;
	rdfs:label "Spatial Measure Component"@en ;
	rdfs:comment "Allows identification of datasets containing spatial location measures"@en ;
	rdfs:subClassOf [
        a owl:Restriction ;
        owl:onProperty qb:measure;
        owl:someValuesFrom qb4st:SpatialMeasure ;
     ]  ;
.

